ch 3 updated

LAMR/User/hello_world.lean
@@ -2,3 +2,428 @@ import Init
 
 #eval "hello world"
 #eval 2 + 2
+
+/- 3.1 Begin -/
+#check (2 + 2 : Nat)
+
+def four : Nat := 2 + 2
+def isOne (x : Nat) : String := if x = 1 then "yes" else "no"
+#check four
+#print four
+
+#check isOne
+#print isOne
+
+def four' := 2 + 2
+def isOne' x := if x = 1 then "yes" else "no"
+
+#eval four
+#eval isOne 3
+#eval isOne 1
+#eval four'
+#eval isOne' 0
+
+#eval IO.println "Hello, world!"
+
+#check 2 + 2 = 4
+#check 2 + 2 < 5
+#check isOne 3 = "no"
+#check 2 + 2 < 5 ∧ isOne 3 = "no"
+
+def Fermat_statement : Prop := ∀ a b c n : Nat, a * b * c ≠ 0 ∧ n > 2 → a^n + b^n ≠ c^n
+
+theorem two_plus_two_is_four : 2 + 2 = 4 := rfl
+theorem Fermat_last_theorem : Fermat_statement := sorry
+
+def foo n := 3 * n + 7
+
+#eval foo 3
+#eval foo (foo 3)
+
+def bar n := foo (foo n) + 3
+
+#eval bar 3
+#eval bar (bar 3)
+
+def printExample : IO Unit:= do
+  IO.println "world"
+  IO.println "hello"
+
+#eval printExample
+
+def factorial : Nat → Nat
+  | 0       => 1
+  | (n + 1) => (n + 1) * factorial n
+
+#eval factorial 10
+#eval factorial 100
+
+def hanoi (numDisks start finish aux : Nat) : IO Unit :=
+  match numDisks with
+  | 0     => pure ()
+  | n + 1 => do
+      hanoi n start aux finish
+      IO.println s!"Move disk {n + 1} from peg {start} to peg {finish}"
+      hanoi n aux finish start
+
+#eval hanoi 7 1 2 3
+
+def addNums : List Nat → Nat
+  | []      => 0
+  | a::as => a + addNums as
+
+#eval addNums [0, 1, 2, 3, 4, 5, 6]
+
+#eval List.range 7
+
+
+section
+open List
+
+#eval range 7
+#eval addNums <| range 7
+#eval map (fun x => x + 3) <| range 7
+#eval foldl (.+.) 0 <| range 7
+
+end
+
+
+def myRange := List.range 7
+#eval myRange.map fun x => x + 3
+
+
+namespace hidden
+
+def reverseAux : List α → List α → List α
+  | [], r => r
+  | (a::l), r => reverseAux l (a::r)
+
+def reverse (as : List α) : List α := reverseAux as []
+
+protected def append (as bs : List α) : List α := reverseAux as.reverse bs
+
+#eval hidden.append [1, 2, 3] [4, 5, 6]
+#eval hidden.append (bs := [1]) (as := [2])
+
+def f (a : Nat) (b : Nat := 0) : Nat := a * a + b
+
+end hidden
+
+partial def gcd m n := if n = 0 then m else gcd n (m % n)
+#eval gcd 45 30
+#eval gcd 37252 49824
+
+partial def bad (n : Nat) : Nat := bad (n + 1)
+
+def fib' : Nat → Nat
+  | 0 => 0
+  | 1 => 1
+  | n + 2 => fib' (n + 1) + fib' n
+
+#eval fib' 5
+
+def fibAux : Nat → Nat × Nat
+  | 0 => (0, 1)
+  | n + 1 => let p := fibAux n; (p.2, p.1 + p.2)
+
+def fib n := (fibAux n).1
+
+#eval (List.range 20).map fib
+
+def fibListAux : Nat → List Nat
+  | 0 => []
+  | 1 => [0]
+  | 2 => [1, 0]
+  | n + 1 => let l := fibListAux n; (l[0]! + l[1]!)::l
+
+def fibList n := (fibListAux n).reverse
+
+#eval fibList 20
+
+#print Option
+
+def bar1 (n? : Option Nat) : Nat :=
+  match n? with
+    | some n => n
+    | none   => 0
+
+#eval bar1 (some 5)
+#eval bar1 none
+#print Option.getD
+#eval (some 5).getD 0
+#eval none.getD 0
+/- 3.3 End -/
+
+/- 3.4 Begin -/
+def showSums : IO Unit := do
+  let mut sum := 0
+  for i in [0:100] do
+    sum := sum + i
+    IO.println s!"i: {i}, sum: {sum}"
+
+#eval showSums
+
+/-QUESTION: the keyword 'return' is not necessary? -/
+/-QUESTION: else-branch is optional? -/
+def isPrime (n : Nat) : Bool := Id.run do
+  if n < 2 then false else
+    for i in [2:n] do
+      if n % i = 0 then
+        return false
+      if i * i > n then
+        return true
+    true
+
+#eval (List.range 10000).filter isPrime
+
+def bar2 (n? : Option Nat) : IO Unit := do
+  let some n := n? |
+    IO.println "oops"
+  IO.println n
+
+#eval bar2 (some 2)
+#eval bar2 none
+
+def primes (n : Nat) : Array Nat := Id.run do
+  let mut result := #[]
+  for i in [2:n] do
+    if isPrime i then
+      result := result.push i
+  result
+
+#eval (primes 10000).size
+
+def a : Array Nat := #[1, 2]
+#print a
+
+def mulTable : Array (Array Nat) := Id.run do
+  let mut table := #[]
+  for i in [:10] do
+    let mut row := #[]
+    for j in [:10] do
+      row := row.push ((i + 1) * (j + 1))
+    table := table.push row
+  table
+
+#eval mulTable
+
+def mulTable' : Array (Array Nat) := Id.run do
+  let mut s := mkArray 10 (mkArray 10 0)
+  for i in [:10] do
+    for j in [:10] do
+      s := s.set! i <| s[i]!.set! j ((i + 1) * (j + 1))
+  s
+
+#eval mulTable'
+
+#eval show IO Unit from do
+  for i in [:10] do
+    for j in [:10] do
+      let numstr := toString mulTable[i]![j]!
+      -- print 1-3 spaces
+      IO.print <| " ".pushn ' ' (3 - numstr.length)
+      IO.print numstr
+    IO.println ""
+/- 3.4 End -/
+
+/- 3.5 Exercises -/
+/-1-/
+def divs (n : Nat) : List Nat := (List.range n).filter (n % . = 0)
+
+/-2-/
+def perfect (n : Nat) : Bool := n = (addNums <| divs n)
+
+def perfects (n : Nat) : List Nat := (List.range n).filter perfect
+#eval perfects 1000
+
+#eval 0::([1, 2] ++ [3])
+
+/-3-/
+def sublists : List α → List (List α)
+  | [] => [[]]
+  | (a::as) => let t := sublists as; t ++ t.map (fun x => a::x)
+
+#eval sublists [1, 2, 3]
+
+/-4-/
+/- by induction. -/
+
+/-5-/
+def insertAux (a : α) (as : List α) : List (List α) :=
+List.map (fun i => as.insertIdx i a) (List.range (as.length + 1))
+
+def f (a : α) : List (List α) → List (List α)
+  | [] => []
+  | bs::bss => (insertAux a bs) ++ f a bss
+
+#eval f 0 [[1, 2], [2, 1]]
+
+def permutations : List α → List (List α)
+  | [] => [[]]
+  | (a::as) => f a <| permutations as
+
+#eval permutations [1, 2, 3]
+
+/-6-/
+/- by induction; inductive step, note that there are n + 1 positions at which an
+element can be inserted into a list of length n -/
+
+/-7-/
+/- not sure why no error when α is instantiated by Nat -/
+def transpose (l : List (List α)) : List (List α) :=
+List.map (fun i => List.map (fun vec => List.get! vec i) l)  (List.range (l.length))
+
+def mat := [[1, 2, 3], [4, 5, 6], [7, 8, 9]]
+#eval transpose mat
+
+/-8-/
+def hanoi8 (numDisks start finish aux : Nat) : IO Unit :=
+  match numDisks with
+    | 0 => pure ()
+    | n + 1 => do
+      if start = 1
+      then if finish = 2
+           then /- finish = 2, aux = 3 -/
+                hanoi8 n start aux finish
+                IO.println s!"Move disk {n + 1} from peg {start} to peg {finish}"
+                hanoi8 n aux finish start
+           else /- finish = 3, aux = 2 -/
+                hanoi8 n start finish aux
+                IO.println s!"Move disk {n + 1} from peg {start} to peg {aux}"
+                hanoi8 n finish start aux
+                IO.println s!"Move disk {n + 1} from peg {aux} to peg {finish}"
+                hanoi8 n start finish aux
+      else if start = 2
+           then if finish = 3
+                then /- finish = 3, aux = 1 -/
+                     hanoi8 n start aux finish
+                     IO.println s!"Move disk {n + 1} from peg {start} to peg {finish}"
+                     hanoi8 n aux finish start
+                else /- finish = 1, aux = 3 -/
+                     hanoi8 n start aux finish
+                     IO.println s!"Move disk {n + 1} from peg {start} to peg {finish}"
+                     hanoi8 n aux finish start
+           else /- start = 3 -/
+                if finish = 1
+                then /- finish = 1, aux = 2 -/
+                     hanoi8 n start finish aux
+                     IO.println s!"Move disk {n + 1} from peg {start} to peg {aux}"
+                     hanoi8 n finish start aux
+                     IO.println s!"Move disk {n + 1} from peg {aux} to peg {finish}"
+                     hanoi8 n start finish aux
+                else /- finish = 2, aux = 1 -/
+                     hanoi8 n start aux finish
+                     IO.println s!"Move disk {n + 1} from peg {start} to peg {finish}"
+                     hanoi8 n aux finish start
+
+#eval hanoi8 3 1 2 3
+
+/-9-/
+def hanoi9 (numDisks start finish aux : Nat) : IO Unit :=
+  match numDisks with
+    | 0 => pure ()
+    | n + 1 => do
+      if start = 1
+      then if finish = 2
+           then /- finish = 2, aux = 3 -/
+                hanoi9 n start aux finish
+                IO.println s!"Move disk {n + 1} from peg {start} to peg {finish}"
+                hanoi9 n aux finish start
+           else /- finish = 3, aux = 2 -/
+                hanoi9 n start finish aux
+                IO.println s!"Move disk {n + 1} from peg {start} to peg {aux}"
+                hanoi9 n finish start aux
+                IO.println s!"Move disk {n + 1} from peg {aux} to peg {finish}"
+                hanoi9 n start finish aux
+      else if start = 2
+      then if finish = 3
+           then /- finish = 3, aux = 1 -/
+                hanoi9 n start aux finish
+                IO.println s!"Move disk {n + 1} from peg {start} to peg {finish}"
+                hanoi9 n aux finish start
+           else /- finish = 1, aux = 3 -/
+                hanoi9 n start finish aux
+                IO.println s!"Move disk {n + 1} from peg {start} to peg {aux}"
+                hanoi9 n finish start aux
+                IO.println s!"Move disk {n + 1} from peg {aux} to peg {finish}"
+                hanoi9 n start finish aux
+      else /- start = 3 -/
+           if finish = 1
+           then /- finish = 1, aux = 2 -/
+                hanoi9 n start aux finish
+                IO.println s!"Move disk {n + 1} from peg {start} to peg {finish}"
+                hanoi9 n aux finish start
+           else /- finish = 2, aux = 1 -/
+                hanoi9 n start finish aux
+                IO.println s!"Move disk {n + 1} from peg {start} to peg {aux}"
+                hanoi9 n finish start aux
+                IO.println s!"Move disk {n + 1} from peg {aux} to peg {finish}"
+                hanoi9 n start finish aux
+
+#eval hanoi9 3 1 2 3
+
+/-10-/
+namespace LbBinTree
+inductive LbBinTree where
+  | empty : LbBinTree
+  | node  : Nat → LbBinTree → LbBinTree → LbBinTree
+  deriving Repr, DecidableEq, Inhabited
+
+def sum : LbBinTree → Nat
+  | LbBinTree.empty => 0
+  | LbBinTree.node n l r => n + sum l + sum r
+
+def lt := LbBinTree.node 5 (LbBinTree.node 3 LbBinTree.empty LbBinTree.empty) (LbBinTree.node 1 (LbBinTree.node 2 LbBinTree.empty LbBinTree.empty) LbBinTree.empty)
+#eval sum lt
+
+def inorder (t : LbBinTree) : IO Unit :=
+  match t with
+    | LbBinTree.empty => pure ()
+    | LbBinTree.node n l r => do
+      inorder l
+      IO.println s!"{n}"
+      inorder r
+
+#eval inorder lt
+
+def preorder (t : LbBinTree) : IO Unit :=
+  match t with
+    | LbBinTree.empty => pure ()
+    | LbBinTree.node n l r => do
+      IO.println s!"{n}"
+      preorder l
+      preorder r
+
+#eval preorder lt
+
+def postorder (t : LbBinTree) : IO Unit :=
+  match t with
+    | LbBinTree.empty => pure ()
+    | LbBinTree.node n l r => do
+      postorder l
+      postorder r
+      IO.println s!"{n}"
+
+#eval postorder lt
+end LbBinTree
+
+/-11-/
+def pascal (n : Nat) : IO Unit :=
+  match n with
+    | 0 => pure ()
+    | m + 1 => do
+      let mut s := mkArray 1 1
+      for i in [:m + 1] do
+        if i ≠ 0 then IO.println ""
+        --print s--
+        for j in [:s.size] do
+          if j ≠ 0 then IO.print ", "
+          IO.print s[j]!
+        --update s--
+        s := s.push 1
+        --s.size - 2, s.size - 3, ..., 2, 1
+        --s.size - 1 - 1, ..., s.size - 1 - (s.size - 2)
+        for j in [1:s.size - 1] do
+          s := s.set! (s.size - 1 - j) (s[s.size - 1 - j]! + s[s.size - 2 - j]!)
+      IO.println ""
+#eval pascal 10
